theories/certs/footer.v
@@ -1,0 +1,28 @@
+Definition sorted_order := Eval compute in sort <%O final_order.
+
+Definition reorderK := @pordK _ final_order sorted_order
+                      is_true_true is_true_true.
+
+Theorem isopres_final : isopres present_entry present_final.
+Proof.
+have wfc : wfpres_cert present_entry cert by vm_cast_no_check (eq_refl true).
+apply: (isopres_trans (@iso_final_pres _ present_entry cert wfc)).
+apply: pres_irrelevance.
+  by rewrite (pgen_final_pres wfc).
+by rewrite (prelat_final_pres wfc).
+Time Qed.
+
+Theorem final_ok : convergent (prelat present_final).
+Proof.
+apply: (rgen_convergent reorderK erefl).
+apply: diamond.
+  apply: (decreasing_wf (@lt_sizelexi_stable _ int) sizelexi_int_wf).
+  by native_cast_no_check (eq_refl true).
+apply: (spair_confluenceP (fuel := 20)).
+rewrite spair_confluence_dec_intE.
+(* Set NativeCompute Timing.
+Set NativeCompute Profiling.
+Time by native_compute.  *)
+by native_cast_no_check (eq_refl true).
+(* Optimize Heap. *)
+Time Qed.
